src/ReactorModel/Objects/Reactor/Theorems/WellIndexable.lean
@@ -5,7 +5,44 @@ namespace ReactorType
 
 class WellIndexable (α) extends Indexable α, WellFounded α
 
-variable [WellIndexable α] {rtr : α}
+variable [WellIndexable α] {rtr₁ : α}
+
+-- TODO: See comments above `StrictMember.rtr_equiv`.
+theorem StrictMember.lawfulMemUpdate_object_preserved 
+    (u : LawfulMemUpdate cpt i f rtr₁ rtr₂) (h : c ≠ cpt ∨ j ≠ i) (s₁ : StrictMember c j rtr₁)
+    (s₂ : StrictMember c j rtr₂) : s₁.object = s₂.object := by
+  induction s₁ generalizing rtr₂ <;> cases s₂ <;> simp [object]
+  case final.final h₁ _ h₂ =>
+    cases u
+    case final e => simp_all [e.valued h]
+    case nested e => simp_all [e (c := c) (.inl $ by simp)]
+  case nested.nested j₁ _ h₁ s₁ hi j₂ _ s₂ h₂ => 
+    have hj : j₁ = j₂ := by 
+      have hs := (nested h₁ s₁ |>.fromEquiv u.equiv).unique (nested h₂ s₂)
+      simp [fromEquiv] at hs
+      exact hs.left
+    subst hj
+    cases u
+    case final e => 
+      cases h₂ ▸ (e (c := .rtr) (j := j₁) (.inl $ by simp)) ▸ h₁
+      simp [s₁.unique s₂]
+    case nested j' _ _ u _ _ e =>
+      by_cases hj : j₁ = j'
+      case neg => 
+        cases h₂ ▸ (e (c := .rtr) (j := j₁) (.inr hj)) ▸ h₁
+        simp [s₁.unique s₂]
+      case pos => 
+        simp_all [hj]
+        exact hi (h₁ ▸ h₂ ▸ u) _
+  case final.nested h₁ _ _ s₂ h₂ =>
+    injection (final h₁ |>.fromEquiv u.equiv).unique (nested h₂ s₂)
+  case nested.final h₁ s₁ _ _ h₂ =>
+    injection (nested h₁ s₁).unique (final h₂ |>.fromEquiv $ ReactorType.Equivalent.symm u.equiv)     
+
+theorem Member.lawfulMemUpdate_object_preserved 
+    (u : LawfulMemUpdate cpt i f rtr₁ rtr₂) (h : c ≠ cpt ∨ j ≠ i) :
+    (m₁ : Member c j rtr₁) → (m₂ : Member c j rtr₂) → m₁.object = m₂.object
+  | .strict s₁, .strict s₂ => s₁.lawfulMemUpdate_object_preserved u h s₂
 
 namespace LawfulMemUpdate
 
@@ -14,13 +51,13 @@ variable [WellIndexable α] {rtr₁ : α}
 
 theorem obj?_some₁ (u : LawfulMemUpdate cpt i f rtr₁ rtr₂) : ∃ o, rtr₁[cpt][i] = some o := by
   induction u 
-  case final         => exact ⟨_, get?_some_to_obj?_some ‹_›⟩
-  case nest h _ _ hi => exact ⟨_, obj?_some_nested h hi.choose_spec⟩
+  case final           => exact ⟨_, get?_some_to_obj?_some ‹_›⟩
+  case nested h _ _ hi => exact ⟨_, obj?_some_nested h hi.choose_spec⟩
 
 theorem obj?_some₂ (u : LawfulMemUpdate cpt i f rtr₁ rtr₂) : ∃ o, rtr₂[cpt][i] = some o := by
   induction u 
-  case final       => exact ⟨_, get?_some_to_obj?_some ‹_›⟩
-  case nest h _ hi => exact ⟨_, obj?_some_nested h hi.choose_spec⟩
+  case final         => exact ⟨_, get?_some_to_obj?_some ‹_›⟩
+  case nested h _ hi => exact ⟨_, obj?_some_nested h hi.choose_spec⟩
 
 theorem obj?_some_iff (u : LawfulMemUpdate cpt i f rtr₁ rtr₂) : 
     (∃ o, rtr₁[c][j] = some o) ↔ (∃ o, rtr₂[c][j] = some o) :=
@@ -30,57 +67,22 @@ theorem obj?_none_iff (u : LawfulMemUpdate cpt i f rtr₁ rtr₂) :
     (rtr₁[c][j] = none) ↔ (rtr₂[c][j] = none) :=
   Equivalent.obj?_none_iff u.equiv
 
-/-
--- TODO: This is a general (perhaps very important) theorem about obj?.
-theorem obj?_some_elim {rtr : α} {i : ID} (h : rtr[cpt][i] = some o) : (rtr{cpt}{i} = some o) ∨ (∃ j con, rtr{.rtr}{j} = some con ∧ con[cpt][i] = some o) :=
-  sorry
-  -- This should be derivable directly from obj?_to_con?_and_cpt?
--/
-
 theorem obj?_preserved (u : LawfulMemUpdate cpt i f rtr₁ rtr₂) (h : c ≠ cpt ∨ j ≠ i) : 
     rtr₂[c][j] = rtr₁[c][j] := by
   cases ho₁ : rtr₁[c][j]
-  case none => sorry -- simp [u.obj?_none_iff.mp ho₁]
+  case none => simp [obj?_none_iff u |>.mp ho₁]
   case some =>
-    sorry
-    /-
-    have ⟨_, ho₂⟩ := u.obj?_some_iff.mp ⟨_, ho₁⟩ 
-    simp [ho₂]
-
-    -- TODO: We need to somehow distinguish whether [c][j] lives in the same reactor as [cpt][i].
-    induction u
-    case final e _ _ =>
-      cases obj?_some_elim ho₁ <;> cases obj?_some_elim ho₂
-      case inl.inl h₁ h₂ =>
-        injection h₁ ▸ h₂ ▸ e (c := c) (j := j) (by simp [h]) with h
-        exact h.symm
-      case inr.inr h₁ h₂ =>
-        obtain ⟨j₁, con₁, hn₁, hc₁⟩ := h₁
-        obtain ⟨j₂, con₂, hn₂, hc₂⟩ := h₂
-        simp at hc₁ hc₂
-        have hj : j₁ = j₂ := sorry 
-        subst hj
-        have hn := e (c := .rtr) (j := j₁) (by simp [h])
-        injection hn₂ ▸ hn ▸ hn₁ with h
-        subst h
-        injection hc₁ ▸ hc₂ with h
-        exact h.symm
-      case inl.inr =>
-        simp at * -- contra
-        sorry
-      case inr.inl =>
-        simp at * -- contra
-        sorry
-    case nest =>
-      sorry
-    -/
+    have ⟨_, ho₂⟩ := obj?_some_iff u |>.mp ⟨_, ho₁⟩ 
+    have ⟨m₁⟩ := Object.iff_obj?_some.mpr ho₁
+    have ⟨m₂⟩ := Object.iff_obj?_some.mpr ho₂
+    simp [ho₂, m₁.lawfulMemUpdate_object_preserved u h m₂]
 
 theorem obj?_updated (u : LawfulMemUpdate cpt i f rtr₁ rtr₂) : 
     rtr₂[cpt][i] = f <$> rtr₁[cpt][i] := by
   induction u
   case final h₁ h₂ => 
     rw [get?_some_to_obj?_some h₁, get?_some_to_obj?_some h₂, Option.map_some]
-  case nest h₁ h₂ u hi =>
+  case nested h₁ h₂ u hi =>
     have ⟨_, h₁'⟩ := u.obj?_some₁
     have ⟨_, h₂'⟩ := u.obj?_some₂
     rw [obj?_some_nested h₁ h₁', obj?_some_nested h₂ h₂']
@@ -99,7 +101,7 @@ theorem obj?_preserved (h : c ≠ cpt ∨ j ≠ i) :
   | notMem _ h => h ▸ rfl
 
 theorem obj?_updated : (LawfulUpdate cpt i f rtr₁ rtr₂) → rtr₂[cpt][i] = f <$> rtr₁[cpt][i]
-  | update u => u.obj?_updated
+  | update u   => u.obj?_updated
   | notMem h e => by subst e; simp [member_isEmpty_obj?_none h]
 
 end LawfulUpdate
